src/goose_lang/lang.v
@@ -19,7 +19,9 @@ operations and crash semantics for foreign operations. See goose_lang/ffi/disk.v
 for our main FFI example.
 
 - Unlike HeapLang, we keep a left-to-right evaluation order to match Go and
-  because curried functions no longer arise.
+  because curried functions no longer arise. (BUG(tej): built-in functions and
+  operators are left-to-right, but function calls are still left-to-right. This
+  should be fixed.)
 - Some support for prophecy variables is retained in case we need it later, but we have no way of inserting these from the source code using Goose and haven't developed reasoning principles
 
 *)
